
				<exercises>
					<p><exercise><!-- xml:id="ex-" -->
						<statement>
							<aside><p> (Source: <xref ref="ref-KN" />, Chapter 2, Exercise 2.1.3) </p></aside>
							Let
							<m> A = \begin{bmatrix} 2 \amp 1 \\ 0 \amp -1 \end{bmatrix},
								B = \begin{bmatrix} 3 \amp -1 \amp 2\\ 0 \amp 1 \amp 4 \end{bmatrix},
								C = \begin{bmatrix} 3 \amp -1 \\ 2 \amp 0 \end{bmatrix},
								D = \begin{bmatrix} 1 \amp 3 \\ -1 \amp 0 \\ 1 \amp 4 \end{bmatrix},</m> and
							<m>
								E = \begin{bmatrix} 1 \amp 0 \amp 1 \\ 0 \amp 1 \amp 0 \end{bmatrix}.
							</m> Compute the following (where possible).
							 <ol cols="3">
								<li>
									<m> 3A - 2B </m>
								</li>
								<li> 
									<m> 5C </m>
								</li>
								<li> 
									<m> 3E^t </m>
								</li>
								<li> 
									<m> B+D </m>
								</li>
								<li>
									<m> 4A^t - 3C </m>
								</li>
								<li>
									<m> (A+C)^t </m>
								</li>
								<li>
									<m> 2B - 3E </m>
								</li>
								<li> 
									<m> A - D </m>
								</li>
								<li>
									<m>(B- 2E)^t </m>
								</li>
							</ol>
						</statement>
						<hint><aside><p> (Source: <xref ref="ref-KN" />, Chapter 2, Definition 2.1) </p></aside>
							Recall: If <m>A</m> and <m>B</m> are matrices of the same size, their <em>sum</em> <m>A+B</m> is the matrix formed by adding corresponding entries.
						</hint>
						<hint><aside><p> (Source: <xref ref="ref-KN" />, Chapter 2, Definition 2.2) </p></aside>
							Recall: If <m>A</m> is any matrix and <m>k</m> is any number, the <em>scalar multiple</em> <m>kA</m> is the matrix obtained from <m>A</m> by multiplying each entry of <m>A</m> by <m>k</m> .
						</hint>
						<hint xml:id="hint-matrix-transpose"><aside><p> (Source: <xref ref="ref-KN" />, Chapter 2, Definition 2.3) </p></aside>
							Recall: If <m>A</m> is a <m>m\times n</m> matrix, the <em>transpose</em> of <m>A</m>, written <m>A^t</m>, is the <m>n\times m</m> matrix whose rows are just the columns of  <m>A</m> in the same order.
						</hint>
						<solution>
							<ol>
								<li><solution>
									We cannot add these matrices as they are not of the same size (<m>3A</m> is a <m>2\times 2</m> matrix, while <m>2B</m> is a <m>2\times 3</m> matrix).
								</solution></li>
								<li><solution> 
									<me> 5C = 5\begin{bmatrix} 3 \amp -1 \\ 2 \amp 0 \end{bmatrix} = \begin{bmatrix} 15 \amp -5 \\ 10 \amp 0 \end{bmatrix}</me>.
								</solution></li>
								<li><solution>
									<me> 3E^t = 3 \begin{bmatrix} 1 \amp 0 \amp 1 \\ 0 \amp 1 \amp 0 \end{bmatrix}^{T}
									=3 \begin{bmatrix} 1 \amp 0  \\  0  \amp 1 \\ 1 \amp 0 \end{bmatrix}
									=
									\begin{bmatrix} 3 \amp 0  \\  0  \amp 3 \\ 3 \amp 0 \end{bmatrix}.
									 </me>
								</solution></li>
								<li><solution> 
									We cannot add these matrices as they are not of the same size (<m>-B</m> is a <m>2\times 3</m> matrix, while <m>D</m> is a <m>3\times 2</m> matrix).
								</solution></li>
								<li><solution>
									<md>
										<mrow>4A^t - 3C \amp = 4 \begin{bmatrix} 2 \amp 1 \\ 0 \amp -1 \end{bmatrix}^t - 3\begin{bmatrix} 3 \amp -1 \\ 2 \amp 0 \end{bmatrix}</mrow>
										<mrow>\amp = 4 \begin{bmatrix} 2 \amp 0 \\ 1 \amp -1 \end{bmatrix} - \begin{bmatrix} 9 \amp -3 \\ 6 \amp 0 \end{bmatrix}</mrow>
										<mrow>\amp = \begin{bmatrix} 8 - 9 \amp 0 - (-3) \\ 4 - 6 \amp -4 - 0 \end{bmatrix}</mrow>										
										<mrow>\amp = \begin{bmatrix} -1 \amp 3 \\ -2 \amp -4 \end{bmatrix}.</mrow>
									</md>
								</solution></li>
								<li><solution>
									<md>
										<mrow>(A+C)^t \amp = \left( \begin{bmatrix} 2 \amp 1 \\ 0 \amp -1 \end{bmatrix} + \begin{bmatrix} 3 \amp -1 \\ 2 \amp 0 \end{bmatrix}\right)^t </mrow>
										<mrow> \amp = \begin{bmatrix} 5 \amp 0 \\ 2 \amp -1 \end{bmatrix}^t </mrow>
										<mrow> \amp = \begin{bmatrix} 5 \amp 2 \\ 0 \amp -1 \end{bmatrix}.</mrow>
									</md>
								</solution></li>
								<li><solution>
									<md>
										<mrow> 2B - 3E \amp = 2 \begin{bmatrix} 3 \amp -1 \amp 2\\ 0 \amp 1 \amp 4 \end{bmatrix} - 3 \begin{bmatrix} 1 \amp 0 \amp 1 \\ 0 \amp 1 \amp 0 \end{bmatrix}</mrow>
										<mrow>\amp = \begin{bmatrix} 6 \amp -2 \amp 4\\ 0 \amp 2 \amp 8 \end{bmatrix}
											- \begin{bmatrix} 3 \amp 0 \amp 3 \\ 0 \amp 3 \amp 0 \end{bmatrix}</mrow>
										<mrow>\amp = \begin{bmatrix} 3 \amp -2 \amp 1\\ 0 \amp -1 \amp 8 \end{bmatrix}.</mrow>
									</md>
								</solution></li>
								<li><solution> 
									We cannot add these matrices as they are not of the same size (<m>A</m> is a <m>2\times 2</m> matrix, while <m>-D</m> is a is a <m>3\times 2</m> matrix).
								</solution></li>
								<li><solution>
									<md>
										<mrow> (B- 2E)^t \amp = \left( \begin{bmatrix} 3 \amp -1 \amp 2\\ 0 \amp 1 \amp 4 \end{bmatrix} - 2 \begin{bmatrix} 1 \amp 0 \amp 1 \\ 0 \amp 1 \amp 0 \end{bmatrix}\right)^{T}</mrow>
										<mrow> \amp = \begin{bmatrix} 3 - 2 \amp -1 - 0 \amp 2 - 2\\ 0 - 0 \amp 1 - 2 \amp 4 - 0 \end{bmatrix}^{T}</mrow>
										<mrow> \amp = \begin{bmatrix} 1 \amp -1 \amp 0\\ 0 \amp -1 \amp 4 \end{bmatrix}^{T}</mrow>
										<mrow> \amp = \begin{bmatrix} 1\amp 0 \\ -1 \amp -1 \\ 0 \amp 4 \end{bmatrix}.</mrow>
									</md>
								</solution></li>
							</ol>
						</solution>
						<answer>
							<ol>
								<li><answer>
									Does not exist.
								</answer></li>
								<li><answer> 
									<me> 5C = \begin{bmatrix} 15 \amp -5 \\ 10 \amp 0 \end{bmatrix}</me>.
								</answer></li>
								<li><answer>
									<me> 3E^t =
									\begin{bmatrix} 3 \amp 0  \\  0  \amp 3 \\ 3 \amp 0 \end{bmatrix}.
									 </me>
								</answer></li>
								<li><answer> 
									Does not exist.
								</answer></li>
								<li><answer>
									<md>
										<mrow>4A^t - 3C \amp = \begin{bmatrix} -1 \amp 3 \\ -2 \amp -4 \end{bmatrix}.</mrow>
									</md>
								</answer></li>
								<li><answer>
									<md>
										<mrow>(A+C)^t \amp = \begin{bmatrix} 5 \amp 2 \\ 0 \amp -1 \end{bmatrix}.</mrow>
									</md>
								</answer></li>
								<li><answer>
									<md>
										<mrow> 2B - 3E \amp = \begin{bmatrix} 3 \amp -2 \amp 1\\ 0 \amp -1 \amp 8 \end{bmatrix}.</mrow>
									</md>
								</answer></li>
								<li><answer> 
									Does not exist.
								</answer></li>
								<li><answer>
									<md>
										<mrow> (B- 2E)^t \amp = \begin{bmatrix} 1\amp 0 \\ -1 \amp -1 \\ 0 \amp 4 \end{bmatrix}.</mrow>
									</md>
								</answer></li>
							</ol>
						</answer>
					</exercise></p>

					

					

					
					<p><exercise><!-- xml:id="ex-" -->
						<statement>
						<aside><p> (Source: <xref ref="ref-KN" />, Chapter 2, Exercise 2.1.5) </p></aside>
						Find <m> A </m> in terms of <m> B </m> if: 
						<ol cols="2">
							<li> 
								<me> A + B = 3A + 2B </me>
							</li>
							<li>
								<me>
									2A - B = 5(A + 2B) </me>
							</li>
						</ol>
					</statement>
						<hint>
							Use the properties from <xref ref="thm-basic-matrix-operation-properties" />.
						</hint>
						<solution>
							Because of the properties listed in <xref ref="thm-basic-matrix-operation-properties" />, we can manipulate both sides of the equations just like we would if <m>A</m> and <m>B</m> were numbers:
							<ol>
							<li> 
								<md>
									<mrow> A + B = 3A + 2B \iff \amp (1-3)A = (2-1)B </mrow>									
									<mrow>\iff \amp -2A = B </mrow>																
									<mrow>\iff \amp A= -\frac{1}{2} B. </mrow>
								</md>
							</li>
							<li>
								<md>
									<mrow>2A - B = 5(A + 2B)  \iff \amp 2A - B = 5A + 10B</mrow>
									<mrow>\iff \amp -3A = 11B</mrow>
									<mrow>\iff \amp A = -\frac{11}{3}B. </mrow>
								</md>
							</li>
						</ol>
						</solution>
						<answer>
							<ol cols="2">
							<li> 
								<me> A= -\frac{1}{2} B  </me>
							</li>
							<li>
								<me>
									A = -\frac{11}{3}B 
								</me>
							</li>
						</ol>
						</answer>
					</exercise></p>
 					<p><exercise><!-- xml:id="ex-" -->
						<statement>
							<aside><p> (Source: <xref ref="ref-KN" />, Chapter 2, Exercise 2.1.6) </p></aside>
							If <m> X, Y, A, </m> and <m> B </m> are matrices of the same size, solve the following systems of equations to obtain <m> X </m> and <m> Y </m> in terms of <m> A </m> and <m> B </m>.
							<ol cols="2">
								<li>
									<md>
										<mrow>
											5X + 3Y  \amp =  A
										</mrow>
										<mrow>
											2X + Y  \amp =  B
										</mrow>
									</md>
								</li>
								<li>
									<md>
										<mrow>
											4X + 3Y  \amp =  A
										</mrow>
										<mrow>
											5X + 4Y  \amp =  B
										</mrow>
									</md>
								</li>
							</ol>
						</statement>
						<hint>
							The properties in <xref ref="thm-basic-matrix-operation-properties" /> justify manipulating these equations as if <m>A,B,X,Y</m> were numbers, <em>as long as we do not divide</em>.
						</hint>
						<solution>
							Because of the properties listed in <xref ref="thm-basic-matrix-operation-properties" />, we can manipulate both sides of the equations just like we would if <m>A, B</m> were numbers and <m>X, Y</m> were variables (however, we cannot simply divide by a matrix!).
							<ol>
								<li> <solution>The system can also be written as
									<me>
										\matr{cc|c}{ 5 \amp 3 \amp A \\ 2 \amp 1 \amp B},
									</me>
									where it is important that we remember that <m>A,B</m> are not numbers, so we cannot divide by them. We row-reduce:
									<md>
										<mrow>\matr{cc|c}{5 \amp 3 \amp A
												\\ 	2 \amp 1 \amp B}
										\underset{5R_{2}}{\overset{2R_{1}}{\longrightarrow}}
										\amp
										\matr{cc|c}{10 \amp 6 \amp 2A
												\\ 	10 \amp 5 \amp 5B}
										\overset{-R_{1}+R_{2}}{\longrightarrow}
										\matr{cc|c}{10 \amp 6 \amp 2A
												\\ 	0 \amp -1 \amp 5B-2A}
										</mrow>
										<mrow>
										\overset{6R_{2}+R_{1}}{\longrightarrow}
										\amp
										\matr{cc|c}{10 \amp 0 \amp 2A + 6 (5B-2A)
												\\ 	0 \amp -1 \amp 5B-2A}
											</mrow><mrow>
										\amp=
										\matr{cc|c}{10 \amp 0 \amp -10A + 30 B
										\\ 	0 \amp -1 \amp 5B-2A}.
										</mrow>
									</md>
									We conclude that <m> X= \frac{1}{10} (-10A + 30 B) = -A + 3 B</m> and <m>Y=-5B+2A</m>.</solution>
								</li>
								<li><solution>The system can also be written as
									<me>
										\matr{cc|c}{ 4 \amp 3 \amp A \\ 5 \amp 4 \amp B},
									</me>
									where it is important that we remember that <m>A,B</m> are not numbers, so we cannot divide by them. We row-reduce:
									<md>
										<mrow>
											\matr{cc|c}{ 4 \amp 3 \amp A
														\\ 5 \amp 4 \amp B}
											\overset{5R_{1}}{\underset{4R_{2}}{\longrightarrow}}
											\amp\matr{cc|c}{ 20 \amp 15 \amp 5A
														\\ 20 \amp 16 \amp 4B}
											\overset{-R_{1}+R_{2}}{\longrightarrow}										
											\matr{cc|c}{ 20 \amp 15 \amp 5A
														\\ 0 \amp 1 \amp 4B-5A}
										</mrow>
										<mrow>
											\overset{-15R_{2}+R_{1}}{\longrightarrow}
											\amp\matr{cc|c}{ 20 \amp 0 \amp 5A-15(4B-5A)
														\\ 0 \amp 1 \amp 4B-5A}
										</mrow>
										<mrow>
											\amp=\matr{cc|c}{ 20 \amp 0 \amp 80A-60B
														\\ 0 \amp 1 \amp 4B-5A}
										</mrow>
									</md>
									We conclude that <m> X= \frac{1}{20} (80A-60B) = 4A - 3 B</m> and <m>Y=4B-5A</m>.</solution>
								</li>
							</ol>
						</solution>
						<answer>
							<ol>
								<li> <answer><m> X= -A + 3 B</m>, <m>Y=-5B+2A</m>.</answer>
								</li>
								<li><answer>
									<m> X= 4A - 3 B</m>, <m>Y=4B-5A</m>
								</answer>
								</li>
							</ol>
						</answer>
					</exercise></p>
						
						
						

					<p><exercise><!-- xml:id="ex-" -->
						<statement>
						<aside><p> (Source: <xref ref="ref-KN" />, Chapter 2, Exercise 2.1.16) </p></aside>
						Let <m> A </m> and <m> B </m> be square matrices of the same size.  Prove each of the following:
						<ol>
							<li>
								If <m> A </m> and <m> B </m> are symmetric, then so is <m> A - B </m>. 
							</li>						
							<li>
								If <m>A</m> is symmetric, then so is <m> kA </m> for any scalar <m> k </m>.
							</li>
						</ol>
					</statement>
					<hint>Recall the definition of <xref ref="def-symmetric" text="custom">symmetric</xref>.</hint>
					<!-- <hint>
						</hint> -->
						<solution>
							<ol>
							<li><solution>
								Let <m>A=[a_{ij}]</m> and <m>B=[b_{ij}]</m>, so that <m>A-B=[a_{ij}-b_{ij}]</m>. Since <m>A=At</m>, we have <m>a_{ij} = a_{ji}</m> for all choices of <m>i,j</m>, and similarly <m>b_{ij} = b_{ji}</m>. Thus,
								<md>
									<mrow>(A-B)^{T} \amp= [a_{ij}-b_{ij}]^{T} = [a_{ji}-b_{ji}] </mrow>
									<mrow>\amp= [a_{ij}-b_{ij}]  =  [a_{ij}]-[b_{ij}]  = A-B,</mrow>
								</md>
								so <m>A-B</m> is symmetric.
							</solution>
						</li>
							<li><solution>
								We need to show that <m>(kA)^{T} = k A</m> to conclude that <m>kA</m> is symmetric. Since equality of matrices is entrywise equality, we will consider their <m>(i,j)</m>-entries:
								<p>Let <m>A=[a_{ij}]</m>. By definition of scalar multiplication, <m>kA=[ka_{ij}]</m>. By definition of the transpose, the <m>(i,j)</m>-entry of <m>(kA)^{T}</m> is therefore <m>ka_{ji}</m> (where we swapped the roles of <m>i</m> and <m>j</m>).</p>
								<p>Since <m>A</m> is symmetric, we know that <m>a_{ij}=a_{ji}</m> for any choice of <m>i,j</m>, so in particular <m>ka_{ij}=ka_{ji}</m> also. This means that the <m>(i,j)</m>-entry of <m>kA</m> (namely <m>ka_{ij}</m>) coincides with the <m>(i,j)</m>-entry of <m>(kA)^{T}</m> (namely <m>ka_{ji}</m>), which shows that <m> k A = (kA)^{T} </m> since they are equal entrywise.</p>
							</solution>
							</li>
						</ol>
						</solution>
				</exercise></p>
						<p><exercise><!-- xml:id="ex-" -->
						<statement>
						<aside><p> (Source: <xref ref="ref-KK" />, Chapter 2, Exercise 2.1.29) </p></aside>
						A square matrix is called <em> skew-symmetric </em> if <m> A^t = -A </m>.  Show that the main diagonal of a skew-symmetric matrix consists of only zeros.
				</statement>
						<hint>
							If <m>A=[a_{ij}]</m>, then the main diagonal consists of every entry of the matrix which is of the form <m> a_{ii} </m>.
						</hint>
						<solution>
							Write <m>A=[a_{ij}]</m>. By assumption, 
							<me>
								[a_{ji}] = A^{t} = -A = [-a_{ij}],
							</me>
							so that <m>a_{ji}=-a_{ij} </m> for all choices of <m>i,j</m>. In particular, if <m>i=j</m>, then <m>a_{ii}=-a_{ii} </m>, so <m>a_{ii}=0</m>.
						</solution>
				</exercise> </p>

				<p><exercise><!-- xml:id="ex-" -->
						<statement>
						<aside><p> (Source: <xref ref="ref-KN" />, Chapter 2, Exercise 2.1.17) </p></aside>
						Show that <m> A + A^t </m> is symmetric for <em> any </em> square matrix <m> A </m>.
				</statement>
						<hint>
							Recall the definition of <xref ref="def-symmetric" text="custom">symmetric</xref>.
						</hint>
						<solution>
							Recall first that <m>(A+B)^t = A^t + B^t</m> for any matrices <m>A, B</m> of the same size. Now, since <m>A</m> is square, <m>A</m> and <m>A^t</m> are of the same size, so we may use this fact for <m>B=A^t</m>:
							<md>
								<mrow> (A+A^t)^t \amp= A^t + (A^t)^t</mrow>
								<mrow> \amp = A^t + A,\qquad\text{ since } (A^t)^t=A</mrow>
								<mrow> \amp = A + A^t,\qquad\text{ since addition is commutative.}</mrow>
							</md>
							This shows that <m>A+A^t</m> is its own transpose, i.e. symmetric.
						</solution>
						<!--<answer>
						</answer> -->

				</exercise> </p>
				</exercises>




		