<exercises>
 	<p><exercise><!-- xml:id="ex-" -->
		<statement>
			<aside><p> (Source: <xref ref="ref-KK" />, Chapter 3, Exercise 3.1.1) </p></aside>
				Let <me> A= \begin{bmatrix} 1 \amp 2 \amp 4 \\ 0 \amp 1 \amp 3\\ -2 \amp 5 \amp 1 \end{bmatrix} </me>. Find the following.
					<ol>
						<li> minor<m>(A)_{11}</m> 
						<hint>
							This is the determinant of the <m> 2 \times 2 </m> matrix which results when the first row and column is deleted from <m> A </m>.
						</hint>
						<answer>
						-14
						</answer>
						<solution>
						minor<m>(A)_{11}</m> is given by finding the determinant of the matrix which results when the first row and column is deleted from <m> A </m>.
						<me> \text{minor}(A)_{11} = \begin{bmatrix} 1 \amp 3 \\ 5 \amp 1 \end{bmatrix}=-14 </me>
						</solution> </li>
						
						<li> minor<m>(A)_{21}</m> 
						<hint>
							This is the determinant of the <m> 2 \times 2 </m> matrix which results when the second row and first column is deleted from <m> A </m>.
						</hint>
						<answer>
						-18
						</answer>
						<solution>
						minor<m>(A)_{11}</m> is given by finding the determinant of the matrix which results when the second row and first column is deleted from <m> A </m>.
						<me>\text{minor}(A)_{11} = \begin{bmatrix} 2 \amp 4 \\ 5 \amp 1 \end{bmatrix} </me>
						</solution>
						</li>
						
						<li> minor<m>(A)_{32}</m> <hint>
							This is the determinant of the <m> 2 \times 2 </m> matrix which results when the third row and second column is deleted from <m> A </m>.
						</hint>
						<answer>
						3
						</answer>
						<solution>
						minor<m>(A)_{11}</m> is given by finding the determinant of the matrix which results when the third row and second column is deleted from <m> A </m>.
						<me>\text{minor}(A)_{11} = \begin{bmatrix} 1 \amp 4 \\ 0 \amp 3 \end{bmatrix} </me>
						</solution>
						</li>
						
						<li> cof<m>(A)_{11}</m> <hint>
							<m>cof(A)_{ij}=(-1)^{i+j}\text{minor}(A)_{ij} </m>
						</hint>
						<answer>
							<m>-14</m>
						</answer>
						<solution>
						<m>cof(A)_{11}=(-1)^{1+1}minor(A)_{11} = -14</m>
						</solution>
						</li>
						
						<li> cof<m>(A)_{21}</m> <hint>
							<m>cof(A)_{ij}=(-1)^{i+j}\text{minor}(A)_{ij} </m>
						</hint>
						<answer>
						18
						</answer>
						<solution>
						<m>cof(A)_{21}=(-1)^{2+1}\text{minor}(A)_{21} = 18</m>
						</solution>
						</li>
						
						<li> cof<m>(A)_{32}</m> <hint>
							<m>cof(A)_{ij}=(-1)^{i+j}\text{minor}(A)_{ij} </m>
						</hint>
						<answer>
						-3
						</answer>
						<solution>
						<m>cof(A)_{32}=(-1)^{3+2}\text{minor}(A)_{21} = -3</m>
						</solution>
						</li>
					</ol>	
						</statement>
						 <hint  xml:id="hint-section-4-2-problem-1-hint"> The determinant of a <m> 2 \times 2 </m> matrix, <m> B </m> is <me> det(B) = b_{11}b_{22}- b_{12}b_{21} </me>.
						</hint> 
						<!-- <solution>
						</solution> -->
						<!--<answer>
						</answer> -->
					</exercise></p>
					<p><exercise><!-- xml:id="ex-" -->
						<statement>
							<aside><p> (Source: <xref ref="ref-KK" />, Chapter 3, Exercise 3.1.4) </p></aside>
							Find the following determinant by expanding along the first row and the second column.
							<me> \begin{vmatrix} 1 \amp 2 \amp 1 \\ 2 \amp 1 \amp 3 \\ 2 \amp 1 \amp 1 \end{vmatrix} </me>
						</statement>
						 <hint xml:id="hint-section-4-2-problem-2-hint-1">
						For a <m>3\times3 </m> matrix,<m> A </m>, expanding along the <m>i</m>th row,
						<me>\det(A) = a_{i1}cof(A)_{i1}+a_{i2}cof(A)_{i2}+a_{i3}cof(A)_{i3}</me>
						</hint> 
						<hint xml:id = "hint-section-4-2-problem-2-hint-2">
						For a <m>3\times3 </m> matrix, <m>A</m>, expanding along the <m>j</m>th column,
						<me>\det(A) = a_{1j}cof(A)_{1j}+a_{2j}cof(A)_{2j}+a_{3j}cof(A)_{3j}</me>
						</hint>
						<answer>
						6
						</answer> 
						 <solution>
						 For a <m>3\times3 </m> matrix, expanding along the <m>1</m>st row,
						<me> cof(A)_{11} = (-1)^{1+1}\begin{vmatrix} 1 \amp 3 \\ 1 \amp 1 \end{vmatrix} =-2 </me>
						<me> cof(A)_{12} = (-1)^{1+2}\begin{vmatrix} 2 \amp 3 \\ 2 \amp 1 \end{vmatrix}=(-1)(-4)=4 </me>
						<me> cof(A)_{13} = (-1)^{1+3}\begin{vmatrix} 2 \amp 1 \\ 2 \amp 1 \end{vmatrix}=(-1)(0)=0 </me>
						<me>\det(A) = a_{11}cof(A)_{11}+a_{12}cof(A)_{12}+a_{13}cof(A)_{13}=(1)(-2) + (2)(4)+ (1)(0)=6 </me>
						For a <m>3\times3 </m> matrix, expanding along the <m>2</m>nd column,
						<me> cof(A)_{12} = (-1)^{1+2}\begin{vmatrix} 2 \amp 3 \\ 2 \amp 1 \end{vmatrix} =(-1)(-4)=4 </me>
						<me> cof(A)_{22} = (-1)^{2+2}\begin{vmatrix} 1 \amp 1 \\ 2 \amp 1 \end{vmatrix}=(-1)=-1 </me>
						<me> cof(A)_{32} = (-1)^{3+2}\begin{vmatrix} 1 \amp 1 \\ 2 \amp 3 \end{vmatrix}=(-1)(1)=-1 </me>
						<me>\det(A) = a_{12}cof(A)_{12}+a_{22}cof(A)_{22}+a_{32}cof(A)_{32}=(2)(4) + (1)(-1)+ (1)(-1)=6 </me>
						</solution> 		
					</exercise></p>
					<p><exercise><!-- xml:id="ex-" -->
						<statement>
							<aside><p> (Source: <xref ref="ref-KK" />, Chapter 3, Exercise 3.1.5) </p></aside>
							Find the following determinant by expanding along the first column and the third row.
							<me> \begin{vmatrix} 1 \amp 2 \amp 1 \\ 1 \amp 0 \amp 1 \\ 2 \amp 1 \amp 1 \end{vmatrix} </me>
						</statement>

						<hint>
						See <xref ref="hint-section-4-2-problem-2-hint-2"/> for the definition of a matrix determinant found by expanding along the jth column.
						</hint>
						<hint>
						See <xref ref="hint-section-4-2-problem-2-hint-1"/> for the definition of a matrix determinant found by expanding along the ith row.
						</hint> 
						<answer>
						-6
						</answer> 
						<solution>
						 For a <m>3\times3 </m> matrix, expanding along the <m>1</m>st column,
						<me> cof(A)_{11} = (-1)^{1+1}\begin{vmatrix} 0 \amp 1 \\ 1 \amp 1 \end{vmatrix} =-1 </me>
						<me> cof(A)_{21} = (-1)^{2+1}\begin{vmatrix} 2 \amp 1 \\ 1 \amp 1 \end{vmatrix}=(-1)(1)=-1 </me>
						<me> cof(A)_{31} = (-1)^{3+1}\begin{vmatrix} 1 \amp 2 \\ 1 \amp 0 \end{vmatrix}=-2 </me>
						<me>\det(A) = a_{11}cof(A)_{11}+a_{21}cof(A)_{21}+a_{31}cof(A)_{31}=(1)(-1) + (1)(-1)+ (2)(-2)=-6 </me>
						For a <m>3\times3 </m> matrix, expanding along the <m>3</m>rd row,
						<me> cof(A)_{31} = (-1)^{3+1}\begin{vmatrix} 2 \amp 1 \\ 0 \amp 1 \end{vmatrix} =-2 </me>
						<me> cof(A)_{32} = (-1)^{3+2}\begin{vmatrix} 1 \amp 1 \\ 1 \amp 1 \end{vmatrix}=0 </me>
						<me> cof(A)_{33} = (-1)^{3+3}\begin{vmatrix} 1 \amp 2 \\ 1 \amp 0 \end{vmatrix}=-2</me>
						<me>\det(A) = a_{12}cof(A)_{12}+a_{22}cof(A)_{22}+a_{32}cof(A)_{32}=(2)(-2) + (1)(0)+ (1)(-2)=-6 </me>
						</solution> 
						
					</exercise></p>
					<p><exercise><!-- xml:id="ex-" -->
						<statement>
							<aside><p> (Source: <xref ref="ref-KK" />, Chapter 3, Exercise 3.1.7) </p></aside>
							Compute the determinant by cofactor expansion.  Pick the easiest row or column to use.
							<me> \begin{vmatrix} 1 \amp 0 \amp 0 \amp 1 \\ 2 \amp 1 \amp 1 \amp 0 \\ 0 \amp 0 \amp 0 \amp 2\\  2 \amp 1 \amp 3 \amp 1 \end{vmatrix} </me>
						</statement>
						<hint>
						For a <m>4\times 4 </m> matrix,<m> A </m>, expanding along the <m>i</m>th row,
						<me>\det(A) = a_{i1}cof(A)_{i1}+a_{i2}cof(A)_{i2}+a_{i3}cof(A)_{i3}+a_{i4}cof(A)_{i4}</me>
						</hint> 
						<answer>
						-4
						</answer>
						 <solution>
						 We choose the third row because this choice gives us the most amount of zeros, which means we have less cofactors to compute.
						 For a <m>4\times 4 </m> matrix,<m> A </m>, expanding along the <m>3</m>rd row,
						<me>\det(A) = a_{31}cof(A)_{31}+a_{32}cof(A)_{32}+a_{33}cof(A)_{33}+a_{34}cof(A)_{34}</me>
						<me>\det(A) = (0)cof(A)_{31}+(0)cof(A)_{32}+(0)cof(A)_{33}+(2)cof(A)_{34}</me>
						<me> cof(A)_{34} = (-1)^{3+4}\begin{vmatrix} 1 \amp 0 \amp 0 \\ 2 \amp 1 \amp 1 \\ 2 \amp 1 \amp 3 \end{vmatrix} </me>
						Let <m> B = \begin{bmatrix} 1 \amp 0 \amp 0 \\ 2 \amp 1 \amp 1 \\ 2 \amp 1 \amp 3 \end{bmatrix} </m>. To find the determinant of <m> B </m> we will
						expand along the first row, since it has the most amount of zeros.  
						<me> det(B) = b_{11}cof(B)_{11} + b_{12}cof(B)_{12} + b_{13}cof(B)_{13} </me>
						<me> det(B) = (1)cof(B)_{11} + (0)cof(B)_{12} + (0)cof(B)_{13} = (1)(-1)^{1+1}\begin{vmatrix}1 \amp 1 \\ 1 \amp 3 \end{vmatrix} = 2 </me>
						<me> cof(A)_{34} = -2 </me> 
						<md>
						<mrow> \det(A) \amp = (0)cof(A)_{31}+(0)cof(A)_{32}+(0)cof(A)_{33}+(2)cof(A)_{34} </mrow>
						<mrow> \amp = (2)(-2) </mrow>
						<mrow> \amp = -4 </mrow> </md>
						</solution> 
						
					</exercise></p>
					<p><exercise><!-- xml:id="ex-" -->
						<statement>
							<aside><p> (Source: <xref ref="ref-KK" />, Chapter 3, Exercise 3.1.11) </p></aside>
							An operation is done to get from the first matrix to the second. Identify what was done and tell how it will affect the value of the determinant.
							<me> \begin{bmatrix}a \amp b \\  c \amp d \end{bmatrix} \to \ldots \to \begin{bmatrix}a \amp b \\  a+c \amp b+d \end{bmatrix} </me>
						</statement>
					 	<hint xml:id="hint-section-4-2-problem-6-hint">
						If a multiple of one row of <m> A </m> is added to a different row (or if a multiple of a column is added
						to a different column), the determinant of the resulting matrix is det <m> A</m>.
						</hint> 
						<answer> The first row is added to the second row.  The determinant of the resulting matrix is the same as the determinant of the original matrix. 
						</answer>
						<!-- <solution>
						</solution> -->
						 
					</exercise></p>
					<p><exercise><!-- xml:id="ex-" -->
						<statement>
							<aside><p> (Source: <xref ref="ref-KK" />, Chapter 3, Exercise 3.1.12) </p></aside>
							An operation is done to get from the first matrix to the second. Identify what was done and tell how it will affect the value of the determinant.
							<me> \begin{bmatrix}a \amp b \\  c \amp d \end{bmatrix} \to \ldots \to \begin{bmatrix}a \amp b \\  2c \amp 2d \end{bmatrix} </me>
						</statement>
						 <hint xml:id= "hint-section-4-2-problem-7-hint"> If a row (or column) of <m> A </m>  is multiplied by a constant <m>u</m>, the determinant of the resulting matrix is <m>u(\det A) </m>.
						</hint> 
						<!-- <solution>
						</solution> -->
						<answer> The second row is multiplied by two.  The determinant of the resulting matrix will be twice as much as the determinant of the original matrix.
						</answer> 
					</exercise></p>
						<p><exercise><!-- xml:id="ex-" -->
						<statement>
							<aside><p> (Source: <xref ref="ref-KN" />, Chapter 3, Exercise 3.1.1) </p></aside>
							Compute the determinants of the following matrices.
							<ol cols="2">
							<li> <m> \begin{bmatrix} \cos(\theta) \amp -\sin(\theta) \\ \sin(\theta) \amp \cos(\theta) \end{bmatrix} </m> </li>
							<li> <m> \begin{bmatrix} 0  \amp a \amp 0 \\ b \amp c \amp d \\ 0 \amp e \amp 0 \end{bmatrix} </m> </li>
							<li> <m> \begin{bmatrix} 0 \amp 0 \amp 0 \amp a \\ 0  \amp 0 \amp b \amp p \\ 0 \amp c \amp q \amp k \\ d \amp s \amp t \amp u \end{bmatrix} </m> </li> 
							</ol>
						</statement>
						 <hint> See hint <xref ref="hint-section-4-2-problem-1-hint"/> forr computing determinants of <m> 2 \times 2 </m> matrices. </hint>
						<hint> See <xref ref="hint-section-4-2-problem-2-hint-1"/> for the definition of a matrix determinant of a 3 <m> \times </m> 3 matrix found by expanding along the ith row. </hint>
						<hint> Let <m> A </m> be an upper or lower triangular matrix. Then <m> det(A) </m> is obtained by taking the product of the entries on the main diagonal. </hint>
						 <hint> 
						 Interchanging two distinct rows (or columns) of <m> A </m> means the determinant of the resulting matrix is − det <m> A </m>. </hint>        
						<answer>
						<ol>
						<li> 1 </li>
						<li> 0 </li>
						<li> abcd </li>
						</ol>
						</answer> 
						<solution>
						<ol> 
						<li> <me> \begin{vmatrix} \cos(\theta) \amp -\sin(\theta) \\ \sin(\theta) \amp \cos(\theta) \end{vmatrix} = \cos(\theta)\cos(\theta)+\sin(\theta)\sin(\theta) =1 </me> </li>
						<li> <me> \begin{vmatrix} 0  \amp a \amp 0 \\ b \amp c \amp d \\ 0 \amp e \amp 0 \end{vmatrix} 
						 = a (-1)^{1+2}\begin{vmatrix}b \amp d \\ 0 \amp 0 \end{vmatrix}
						= a (-1) (0) =0 </me> </li>

						<li> We wish to interchange two rows in order to get an upper triangular matrix.  If we interchange two rows, then we must multiply the determinant of the resulting matrix by (-1) twice.  Once we have obtained an upper triangular matrix, we multiply the diagonal elements to get the determinant.
						 
						 <me> \begin{vmatrix} 0 \amp 0 \amp 0 \amp a \\ 0  \amp 0 \amp b \amp p \\ 0 \amp c \amp q \amp k \\ d \amp s \amp t \amp u \end{vmatrix} = (-1)^2 \begin{vmatrix} d \amp s \amp t \amp u \\  0 \amp c \amp q \amp k \\ 0  \amp 0 \amp b \amp p \\  0 \amp 0 \amp 0 \amp a \end{vmatrix}  = abcd </me> </li>
						</ol>
						</solution>
						
					</exercise></p>
					<p><exercise><!-- xml:id="ex-" -->
						<statement>
							<aside><p> (Source: <xref ref="ref-KN" />, Chapter 3, Exercise 3.1.6) </p></aside>
							Evaluate by cursory inspection:
							<ol cols="1">
							<li> <m>\det \begin{bmatrix} a \amp b \amp c \\ a+1 \amp b+1 \amp c+1 \\ a-1 \amp b-1 \amp c-1 \end{bmatrix}</m> 
							<answer>
						0
						</answer>
						<solution>
						We subtract the first row from both the second and third row.
						<me>  \begin{bmatrix} a \amp b \amp c \\ a+1 \amp b+1 \amp c+1 \\ a-1 \amp b-1 \amp c-1 \end{bmatrix}   \to  \begin{bmatrx} a \amp b \amp c \\ 1 \amp 1 \amp 1 \\ -1 \amp -1 \amp -1 \end{bmatrix} </me> 
						Then we multiply the third row by -1 to obtain a matrix which has two rows that are the same.  Hence, the determinant of the original matrix would be (-1)(0) =0. 
						<me>  \begin{vmatrix} a \amp b \amp c \\ a+1 \amp b+1 \amp c+1 \\ a-1 \amp b-1 \amp c-1 \end{vmatrix}=0  </me>
						</solution> 
							</li>
							<li> <m>\det \begin{bmatrix} a \amp b \amp c \\ a+b \amp 2b \amp c+b \\ 2 \amp 2 \amp 2 \end{bmatrix} </m> </li>
							</ol>
						</statement>
						 <hint>  See <xref ref="hint-section-4-2-problem-6-hint"/> for the determinant of the resulting matrix when adding/subtracting two rows.
						</hint> 
						<hint>
						See <xref ref="hint-section-4-2-problem-7-hint"/> for the determinant of the resulting matrix when multiplying a row by a constant.
						</hint>
						<hint>
						If two distinct rows (or columns) of A are identical, det <m>A = 0 </m>
						</hint>
						
						            
					</exercise></p>
					<p><exercise><!-- xml:id="ex-" -->
						<statement>
							<aside><p> (Source: <xref ref="ref-KN" />, Chapter 3, Exercise 3.1.15) </p></aside>
							<ol> 
							<li> Find <m> b </m> if <m>det \begin{bmatrix} 5 \amp -1 \amp x \\ 2 \amp 6 \amp y \\ -5 \amp 4 \amp x \end{bmatrix} = ax + by.</m> 
							<answer><m>b=-15</m></answer>
							<solution> There are many ways to go about finding <m>b</m>, you may expand along various rows or columns.  For this solution, let us expand along the first row. 
							<md> 
								<mrow> det(A) \amp = 5 \begin{vmatrix}6 \amp y \\ 4 \amp x \end{vmatrix} + 1 \begin{vmatrix} 2 \amp y \\ -5 \amp x \end{vmatrix} + x \begin{vmatrix} 2 \amp 6 \\ -5 \amp 4 \end{vmatrix}</mrow>
							<mrow>
								\amp = 5(6x-4y) + (2x+5y) + x(8 + 30) 
							</mrow>
							<mrow> \amp = 30x - 20y+ 2x+5y+38x</mrow>
							<mrow>\amp = 70x - 15y</mrow>
							</md>
							If <m> det(A) = ax + by</m>, then <m>b = -15</m>
							</solution>
						</li>
							<li> Find <m> c </m> if <m>det \begin{bmatrix} 2 \amp x \amp -1 \\ 1 \amp y \amp 3 \\ -3 \amp z \amp 4  \end{bmatrix} = ax + by+cz.</m>
							<answer><m>c = -7</m></answer>
							<solution> As in the previous part (a), there are many ways to go about finding the answer by expanding along various rows or columns.  In this solution, we will expand along the first column.
							<md> 
								<mrow> det(A) \amp = 2 \begin{vmatrix}y \amp 3 \\ z \amp 4 \end{vmatrix} -1 \begin{vmatrix} x \amp -1 \\ z \amp 4 \end{vmatrix} -3 \begin{vmatrix} x \amp -1 \\ y \amp 3 \end{vmatrix}</mrow>
							<mrow>
								\amp = 2(4y-3z) - (4x+z) + -3(3x + y) 
							</mrow>
							<mrow> \amp = 8y-6z-4x-z-9x-3y</mrow>
							<mrow>\amp = -13x +5y-7z</mrow>
							</md>
							If <m> det(A) = ax + by+cz</m>, then <m>c = -7</m>
							</solution>
							</li>
							</ol>
						</statement>
						<hint> See <xref ref="hint-section-4-2-problem-2-hint-1"/> for the definition of a matrix determinant of a 3 <m> \times </m> 3 matrix found by expanding along the ith row. </hint>
						<hint>See <xref ref="hint-section-4-2-problem-2-hint-2"/> for the definition of a matrix determinant found by expanding along the jth column.</hint>
						<hint> See hint <xref ref="hint-section-4-2-problem-1-hint"/> for computing determinants of <m> 2 \times 2 </m> matrices. </hint>
					</exercise></p>
					<p><exercise><!-- xml:id="ex-" -->
						<statement>
							<aside><p> (Source: <xref ref="ref-KK" />, Chapter 3, Exercise 3.1.17) </p></aside>
							Is it true that <m> det(A+B) = det(A)+det(B) </m>? If this is so, explain why. If it is not so, give a counter example.
						</statement>
						<hint> Consider a <m> 2 \times 2 </m> matrix with positive entries and another with negative entries.
						</hint>
						<answer>
							There exists matrices <m>A</m> and <m>B</m> such that <m>det(A+B) \ne det(A) + det(B)</m> and so the statement of the exercise is false.
						</answer>
						<solution>
							There exists matrices <m>A</m> and <m>B</m> such that <m>det(A+B) \ne det(A) + det(B)</m> and so the statement of the exercise is false.  We can show this witha counterexample.
							Let <m> A </m> be the identity matrix, <m> A = \begin{bmatrix} 1 \amp 0 \\ 0 \amp 1 \end{bmatrix}</m> and let <m> B = \begin{bmatrix} -1 \amp 0 \\ 0 \amp -1</m>, then
							<me> det(A+B) = det\left(\begin{bmatrix} 1 \amp 0 \\ 0 \amp 1 \end{bmatrix} + \begin{bmatrix} -1 \amp 0 \\ 0 \amp -1 \end{bmatrix}right) = det(\begin{bmatrix} 0 \amp 0 \\ 0 \amp 0 \end{bmatrix} \ne det(A) + det(B) = 1 + 1 =2 </me> 
						</solution>
						
					</exercise></p>
					<p><exercise><!-- xml:id="ex-" -->
						<statement>
							<aside><p> (Source: <xref ref="ref-KN" />, Chapter 3, Exercise 3.2.2) </p></aside>
							Use determinants to find which real values of c make each of the following matrices invertible.
							<ol cols="2">
							<li> <m> \begin{bmatrix} 1 \amp 0 \amp 3 \\ 3  \amp -4 \amp c \\ 2 \amp 5 \amp 8 \end{bmatrix} </m></li>
							<li> <m> \begin{bmatrix} 0 \amp c \amp -c \\ -1  \amp 2 \amp 1 \\ c \amp -c \amp c \end{bmatrix} </m> </li>
							<li> <m>\begin{bmatrix} c \amp 1 \amp 0 \\ 0  \amp 2 \amp c \\ -1 \amp c \amp 5 \end{bmatrix} </m> </li>
							<li> <m>\begin{bmatrix} 4 \amp c \amp 3 \\ c  \amp 2 \amp c \\ 5 \amp c \amp 4 \end{bmatrix}</m> </li>
							<li> <m>\begin{bmatrix} 1 \amp 2 \amp -1 \\ 0  \amp -1 \amp c \\ 2 \amp c \amp 1 \end{bmatrix} </m></li>
							<li> <m>\begin{bmatrix} 1 \amp c \amp -1 \\ c  \amp 1 \amp 1 \\ 0 \amp 1 \amp c \end{bmatrix} </m></li>
							</ol>
						</statement>
						<!-- <hint>
						</hint> -->
						<!-- <solution>
						</solution> -->
						<!--<answer>
						</answer> -->
					</exercise></p>
	</exercises>